src/program_proof/mvcc/gc_proof.v
@@ -1,0 +1,21 @@
+(* Import definitions/theorems of the Perennial framework with the disk FFI. *)
+From Perennial.program_proof Require Export disk_prelude.
+(* Import Coq model of our Goose program. *)
+From Goose.github_com.mit_pdos.go_mvcc Require Import gc.
+From Perennial.program_proof.mvcc Require Import mvcc_ghost index_proof.
+
+Section heap.
+Context `{!heapGS Σ, !mvcc_ghostG Σ}.
+
+Definition is_gc (gc : loc) (γ : mvcc_names) : iProp Σ := True.
+
+(*****************************************************************)
+(* func MkGC() *GC                                               *)
+(*****************************************************************)
+Theorem wp_MkGC (idx : loc) γ :
+  {{{ True }}}
+    MkGC #idx
+  {{{ (gc : loc), RET #gc; is_gc gc γ }}}.
+Admitted.
+
+End heap.
